x86/Asmgenproof1.v
@@ -86,7 +86,7 @@ Ltac Simplifs := repeat Simplif.
 Section CONSTRUCTORS.
 
 Variable init_sup: sup.
-Variable ge: Genv.symtbl.
+Variable ge: genv.
 Variable fn: function.
 Variable instr_size : instruction -> Z.
 (** Smart constructor for moves. *)
@@ -95,11 +95,7 @@ Lemma mk_mov_correct:
   forall rd rs k c rs1 m,
   mk_mov rd rs k = OK c ->
   exists rs2,
-<<<<<<< HEAD
-     exec_straight init_sup ge fn c rs1 m k rs2 m
-=======
-     exec_straight instr_size ge fn c rs1 m k rs2 m
->>>>>>> origin/StackAware-new
+     exec_straight instr_size init_sup ge fn c rs1 m k rs2 m
   /\ rs2#rd = rs1#rs
   /\ forall r, data_preg r = true -> r <> rd -> rs2#r = rs1#r.
 Proof.
@@ -202,11 +198,7 @@ Lemma mk_shrximm_correct:
   mk_shrximm n k = OK c ->
   Val.shrx (rs1#RAX) (Vint n) = Some v ->
   exists rs2,
-<<<<<<< HEAD
-     exec_straight init_sup ge fn c rs1 m k rs2 m
-=======
-     exec_straight instr_size ge fn c rs1 m k rs2 m
->>>>>>> origin/StackAware-new
+     exec_straight instr_size init_sup ge fn c rs1 m k rs2 m
   /\ rs2#RAX = v
   /\ forall r, data_preg r = true -> r <> RAX -> r <> RCX -> rs2#r = rs1#r.
 Proof.
@@ -250,11 +242,7 @@ Lemma mk_shrxlimm_correct:
   mk_shrxlimm n k = OK c ->
   Val.shrxl (rs1#RAX) (Vint n) = Some v ->
   exists rs2,
-<<<<<<< HEAD
-     exec_straight init_sup ge fn c rs1 m k rs2 m
-=======
-     exec_straight instr_size ge fn c rs1 m k rs2 m
->>>>>>> origin/StackAware-new
+     exec_straight instr_size init_sup ge fn c rs1 m k rs2 m
   /\ rs2#RAX = v
   /\ forall r, data_preg r = true -> r <> RAX -> r <> RDX -> rs2#r = rs1#r.
 Proof.
@@ -292,15 +280,9 @@ Lemma mk_intconv_correct:
   forall mk sem rd rs k c rs1 m,
   mk_intconv mk rd rs k = OK c ->
   (forall c rd rs r m,
-<<<<<<< HEAD
-   exec_instr init_sup ge c (mk rd rs) r m = Next (nextinstr (r#rd <- (sem r#rs))) m) ->
+   exec_instr instr_size init_sup ge c (mk rd rs) r m = Next (nextinstr (Ptrofs.repr (instr_size (mk rd rs)))(r#rd <- (sem r#rs))) m) ->
   exists rs2,
-     exec_straight init_sup ge fn c rs1 m k rs2 m
-=======
-   exec_instr instr_size ge c (mk rd rs) r m = Next (nextinstr (Ptrofs.repr (instr_size (mk rd rs)))(r#rd <- (sem r#rs))) m) ->
-  exists rs2,
-     exec_straight instr_size ge fn c rs1 m k rs2 m
->>>>>>> origin/StackAware-new
+     exec_straight instr_size init_sup ge fn c rs1 m k rs2 m
   /\ rs2#rd = sem rs1#rs
   /\ forall r, data_preg r = true -> r <> rd -> r <> RAX -> rs2#r = rs1#r.
 Proof.
@@ -331,11 +313,7 @@ Lemma mk_storebyte_correct:
   mk_storebyte addr r k = OK c ->
   Mem.storev Mint8unsigned m1 (eval_addrmode ge addr rs1) (rs1 r) = Some m2 ->
   exists rs2,
-<<<<<<< HEAD
-     exec_straight init_sup ge fn c rs1 m1 k rs2 m2
-=======
-     exec_straight instr_size ge fn c rs1 m1 k rs2 m2
->>>>>>> origin/StackAware-new
+     exec_straight instr_size init_sup ge fn c rs1 m1 k rs2 m2
   /\ forall r, data_preg r = true -> preg_notin r (if Archi.ptr64 then nil else AX :: CX :: nil) -> rs2#r = rs1#r.
 Proof.
   unfold mk_storebyte; intros.
@@ -410,11 +388,7 @@ Lemma loadind_correct:
   loadind base ofs ty dst k = OK c ->
   Mem.loadv (chunk_of_type ty) m (Val.offset_ptr rs#base ofs) = Some v ->
   exists rs',
-<<<<<<< HEAD
-     exec_straight init_sup ge fn c rs m k rs' m
-=======
-     exec_straight instr_size ge fn c rs m k rs' m
->>>>>>> origin/StackAware-new
+     exec_straight instr_size init_sup ge fn c rs m k rs' m
   /\ rs'#(preg_of dst) = v
   /\ forall r, data_preg r = true -> r <> preg_of dst -> rs'#r = rs#r.
 Proof.
@@ -467,11 +441,7 @@ Lemma storeind_correct:
   storeind src base ofs ty k = OK c ->
   Mem.storev (chunk_of_type ty) m (Val.offset_ptr rs#base ofs) (rs#(preg_of src)) = Some m' ->
   exists rs',
-<<<<<<< HEAD
-     exec_straight init_sup ge fn c rs m k rs' m'
-=======
-     exec_straight instr_size ge fn c rs m k rs' m'
->>>>>>> origin/StackAware-new
+     exec_straight instr_size init_sup ge fn c rs m k rs' m'
   /\ forall r, data_preg r = true -> preg_notin r (destroyed_by_setstack ty) -> rs'#r = rs#r.
 Proof.
   unfold storeind; intros.
@@ -985,11 +955,7 @@ Lemma transl_cond_correct:
   forall cond args k c rs m,
   transl_cond cond args k = OK c ->
   exists rs',
-<<<<<<< HEAD
-     exec_straight init_sup ge fn c rs m k rs' m
-=======
-     exec_straight instr_size ge fn c rs m k rs' m
->>>>>>> origin/StackAware-new
+     exec_straight instr_size init_sup ge fn c rs m k rs' m
   /\ match eval_condition cond (map rs (map preg_of args)) m with
      | None => True
      | Some b => eval_extcond (testcond_for_condition cond) rs' = Some b
@@ -1150,11 +1116,7 @@ Qed.
 Lemma mk_setcc_base_correct:
   forall cond rd k rs1 m,
   exists rs2,
-<<<<<<< HEAD
-  exec_straight init_sup ge fn (mk_setcc_base cond rd k) rs1 m k rs2 m
-=======
-  exec_straight instr_size ge fn (mk_setcc_base cond rd k) rs1 m k rs2 m
->>>>>>> origin/StackAware-new
+  exec_straight instr_size init_sup ge fn (mk_setcc_base cond rd k) rs1 m k rs2 m
   /\ rs2#rd = Val.of_optbool(eval_extcond cond rs1)
   /\ forall r, data_preg r = true -> r <> RAX /\ r <> RCX -> r <> rd -> rs2#r = rs1#r.
 Proof.
@@ -1234,11 +1196,7 @@ Qed.
 Lemma mk_setcc_correct:
   forall cond rd k rs1 m,
   exists rs2,
-<<<<<<< HEAD
-  exec_straight init_sup ge fn (mk_setcc cond rd k) rs1 m k rs2 m
-=======
-  exec_straight instr_size ge fn (mk_setcc cond rd k) rs1 m k rs2 m
->>>>>>> origin/StackAware-new
+  exec_straight instr_size init_sup ge fn (mk_setcc cond rd k) rs1 m k rs2 m
   /\ rs2#rd = Val.of_optbool(eval_extcond cond rs1)
   /\ forall r, data_preg r = true -> r <> RAX /\ r <> RCX -> r <> rd -> rs2#r = rs1#r.
 Proof.
@@ -1273,11 +1231,7 @@ Lemma mk_sel_correct:
   | None => True
   end ->
   exists rs',
-<<<<<<< HEAD
-     exec_straight init_sup ge fn c rs m k rs' m
-=======
-     exec_straight instr_size ge fn c rs m k rs' m
->>>>>>> origin/StackAware-new
+     exec_straight instr_size init_sup ge fn c rs m k rs' m
   /\ Val.lessdef (Val.select ob rs#rd rs#r2 ty) rs'#rd
   /\ forall r, data_preg r = true -> r <> rd -> rs'#r = rs r.
 Proof.
@@ -1323,11 +1277,7 @@ Lemma transl_sel_correct:
   forall ty cond args rd r2 k c rs m,
   transl_sel cond args rd r2 k = OK c ->
   exists rs',
-<<<<<<< HEAD
-     exec_straight init_sup ge fn c rs m k rs' m
-=======
-     exec_straight instr_size ge fn c rs m k rs' m
->>>>>>> origin/StackAware-new
+     exec_straight instr_size init_sup ge fn c rs m k rs' m
   /\ Val.lessdef (Val.select (eval_condition cond (map rs (map preg_of args)) m) rs#rd rs#r2 ty) rs'#rd
   /\ forall r, data_preg r = true -> r <> rd -> rs'#r = rs r.
 Proof.
@@ -1372,11 +1322,7 @@ Lemma transl_op_correct:
   transl_op op args res k = OK c ->
   eval_operation ge (rs#RSP) op (map rs (map preg_of args)) m = Some v ->
   exists rs',
-<<<<<<< HEAD
-     exec_straight init_sup ge fn c rs m k rs' m
-=======
-     exec_straight instr_size ge fn c rs m k rs' m
->>>>>>> origin/StackAware-new
+     exec_straight instr_size init_sup ge fn c rs m k rs' m
   /\ Val.lessdef v rs'#(preg_of res)
   /\ forall r, data_preg r = true -> r <> preg_of res -> preg_notin r (destroyed_by_op op) -> rs' r = rs r.
 Proof.
@@ -1384,19 +1330,11 @@ Transparent destroyed_by_op.
   intros until v; intros TR EV.
   assert (SAME:
   (exists rs',
-<<<<<<< HEAD
-     exec_straight init_sup ge fn c rs m k rs' m
+     exec_straight instr_size init_sup ge fn c rs m k rs' m
   /\ rs'#(preg_of res) = v
   /\ forall r, data_preg r = true -> r <> preg_of res -> preg_notin r (destroyed_by_op op) -> rs' r = rs r) ->
   exists rs',
-     exec_straight init_sup ge fn c rs m k rs' m
-=======
-     exec_straight instr_size ge fn c rs m k rs' m
-  /\ rs'#(preg_of res) = v
-  /\ forall r, data_preg r = true -> r <> preg_of res -> preg_notin r (destroyed_by_op op) -> rs' r = rs r) ->
-  exists rs',
-     exec_straight instr_size ge fn c rs m k rs' m
->>>>>>> origin/StackAware-new
+     exec_straight instr_size init_sup ge fn c rs m k rs' m
   /\ Val.lessdef v rs'#(preg_of res)
   /\ forall r, data_preg r = true -> r <> preg_of res -> preg_notin r (destroyed_by_op op) -> rs' r = rs r).
   {
@@ -1577,11 +1515,7 @@ Lemma transl_load_correct:
   eval_addressing ge (rs#RSP) addr (map rs (map preg_of args)) = Some a ->
   Mem.loadv chunk m a = Some v ->
   exists rs',
-<<<<<<< HEAD
-     exec_straight init_sup ge fn c rs m k rs' m
-=======
-     exec_straight instr_size ge fn c rs m k rs' m
->>>>>>> origin/StackAware-new
+     exec_straight instr_size init_sup ge fn c rs m k rs' m
   /\ rs'#(preg_of dest) = v
   /\ forall r, data_preg r = true -> r <> preg_of dest -> rs'#r = rs#r.
 Proof.
@@ -1661,11 +1595,7 @@ Lemma transl_store_correct:
   eval_addressing ge (rs#RSP) addr (map rs (map preg_of args)) = Some a ->
   Mem.storev chunk m a (rs (preg_of src)) = Some m' ->
   exists rs',
-<<<<<<< HEAD
-     exec_straight init_sup ge fn c rs m k rs' m'
-=======
-     exec_straight instr_size ge fn c rs m k rs' m'
->>>>>>> origin/StackAware-new
+     exec_straight instr_size init_sup ge fn c rs m k rs' m'
   /\ forall r, data_preg r = true -> preg_notin r (destroyed_by_store chunk addr) -> rs'#r = rs#r.
 Proof.
   unfold transl_store; intros. monadInv H.
